theories/saturn/mpsc_queue_1.v
@@ -69,8 +69,8 @@ Section mpsc_queue_1_G.
     mono_list_auth γ_history (DfracOwn 1) hist.
   #[local] Definition mpsc_queue_1_history_auth γ hist :=
     mpsc_queue_1_history_auth' γ.(mpsc_queue_1_meta_history) hist.
-  #[local] Definition mpsc_queue_1_history_elem γ i node :=
-    mono_list_elem γ.(mpsc_queue_1_meta_history) i node.
+  #[local] Definition mpsc_queue_1_history_at γ i node :=
+    mono_list_at γ.(mpsc_queue_1_meta_history) i node.
 
   #[local] Definition mpsc_queue_1_model₁' γ_model vs :=
     twins_twin1 γ_model (DfracOwn 1) vs.
@@ -132,19 +132,19 @@ Section mpsc_queue_1_G.
   Proof.
     apply mono_list_alloc.
   Qed.
-  #[local] Lemma mpsc_queue_1_history_elem_get {γ hist} i node :
+  #[local] Lemma mpsc_queue_1_history_at_get {γ hist} i node :
     hist !! i = Some node →
     mpsc_queue_1_history_auth γ hist ⊢
-    mpsc_queue_1_history_elem γ i node.
+    mpsc_queue_1_history_at γ i node.
   Proof.
-    setoid_rewrite mono_list_lb_get. apply mono_list_elem_get.
+    apply mono_list_at_get.
   Qed.
   #[local] Lemma mpsc_queue_1_history_agree γ hist i node :
     mpsc_queue_1_history_auth γ hist -∗
-    mpsc_queue_1_history_elem γ i node -∗
+    mpsc_queue_1_history_at γ i node -∗
     ⌜hist !! i = Some node⌝.
   Proof.
-    apply mono_list_lookup.
+    apply mono_list_at_valid.
   Qed.
   #[local] Lemma mpsc_queue_1_history_update {γ hist} node :
     mpsc_queue_1_history_auth γ hist ⊢ |==>
@@ -177,13 +177,13 @@ Section mpsc_queue_1_G.
     apply twins_update'.
   Qed.
 
-  #[local] Lemma mpsc_queue_1_inv_inner_history_elem ι l γ front :
+  #[local] Lemma mpsc_queue_1_inv_inner_history_at ι l γ front :
     inv ι (mpsc_queue_1_inv_inner l γ) -∗
     l.[front] ↦{#3/4} #front ={⊤}=∗
       ∃ i,
       l.[front] ↦{#3/4} #front ∗
       front ↦ₕ Header §Node 2 ∗
-      mpsc_queue_1_history_elem γ i front.
+      mpsc_queue_1_history_at γ i front.
   Proof.
     iIntros "#Hinv Hl_front_1".
     iInv "Hinv" as "(%hist & %past & %_front & %nodes & %back & %vs & >%Hhist & >%Hback & >Hl_front_2 & Hl_back & Hhist & >Hheaders & Hnodes & >Hhistory_auth & Hmodel₂)".
@@ -191,7 +191,7 @@ Section mpsc_queue_1_G.
     assert (hist !! (length past) = Some front) as Hlookup.
     { rewrite Hhist list_lookup_middle //. }
     iDestruct (big_sepL_lookup with "Hheaders") as "#Hfront_hdr"; first done.
-    iDestruct (mpsc_queue_1_history_elem_get (length past) front with "Hhistory_auth") as "#Hhistory_elem"; first done.
+    iDestruct (mpsc_queue_1_history_at_get (length past) front with "Hhistory_auth") as "#Hhistory_at"; first done.
     iSplitR "Hl_front_1"; first iSteps.
     iSteps.
   Qed.
@@ -251,7 +251,7 @@ Section mpsc_queue_1_G.
     {{{ front i,
       RET #front;
       front ↦ₕ Header §Node 2 ∗
-      mpsc_queue_1_history_elem γ i front
+      mpsc_queue_1_history_at γ i front
     }}}.
   Proof.
     iIntros "%Φ #Hinv HΦ".
@@ -261,7 +261,7 @@ Section mpsc_queue_1_G.
     assert (hist !! (length past) = Some front) as Hlookup.
     { rewrite Hhist list_lookup_middle //. }
     iDestruct (big_sepL_lookup with "Hheaders") as "#Hfront_hdr"; first done.
-    iDestruct (mpsc_queue_1_history_elem_get _ front with "Hhistory_auth") as "#Hhistory_elem"; first done.
+    iDestruct (mpsc_queue_1_history_at_get _ front with "Hhistory_auth") as "#Hhistory_at"; first done.
     iSplitR "HΦ"; first iSteps.
     iSteps.
   Qed.
@@ -274,7 +274,7 @@ Section mpsc_queue_1_G.
     {{{ back i,
       RET #back;
       back ↦ₕ Header §Node 2 ∗
-      mpsc_queue_1_history_elem γ i back
+      mpsc_queue_1_history_at γ i back
     }}}.
   Proof.
     iIntros "%Φ #Hinv HΦ".
@@ -283,7 +283,7 @@ Section mpsc_queue_1_G.
     wp_load.
     pose proof Hback as (i & Hlookup)%elem_of_list_lookup.
     iDestruct (big_sepL_lookup with "Hheaders") as "#Hback_hdr"; first done.
-    iDestruct (mpsc_queue_1_history_elem_get with "Hhistory_auth") as "#Hhistory_elem_back"; first done.
+    iDestruct (mpsc_queue_1_history_at_get with "Hhistory_auth") as "#Hhistory_at_back"; first done.
     iSplitR "HΦ"; first iSteps.
     iSteps.
   Qed.
@@ -299,7 +299,7 @@ Section mpsc_queue_1_G.
     {{{
       meta l nroot γ ∗
       inv ι (mpsc_queue_1_inv_inner l γ) ∗
-      mpsc_queue_1_history_elem γ i node ∗
+      mpsc_queue_1_history_at γ i node ∗
       if decide (op = MpscQueue1Other) then True else
         l.[front] ↦{#3/4} #node ∗
         atomic_update (TA := [tele vs]) (TB := TB) (⊤ ∖ ↑ι) ∅ (tele_app $ mpsc_queue_1_model #l) β Ψ ∗
@@ -323,7 +323,7 @@ Section mpsc_queue_1_G.
         ∃ node',
         ⌜res = #node'⌝ ∗
         node' ↦ₕ Header §Node 2 ∗
-        mpsc_queue_1_history_elem γ (S i) node' ∗
+        mpsc_queue_1_history_at γ (S i) node' ∗
         if decide (op = MpscQueue1Other) then True else
           l.[front] ↦{#3/4} #node ∗
           if decide (op = MpscQueue1IsEmpty) then
@@ -333,17 +333,17 @@ Section mpsc_queue_1_G.
       )
     }}}.
   Proof.
-    iIntros "%Φ (#Hmeta & #Hinv & #Hhistory_elem & Hop) HΦ".
+    iIntros "%Φ (#Hmeta & #Hinv & #Hhistory_at & Hop) HΦ".
 
     iInv "Hinv" as "(%hist & %past & %front & %nodes & %back & %vs & >%Hhist & >%Hback & Hl_front_2 & Hl_back & Hhist & Hheaders & Hnodes & >Hhistory_auth & Hmodel₂)".
-    iDestruct (mpsc_queue_1_history_agree with "Hhistory_auth Hhistory_elem") as %Hlookup.
+    iDestruct (mpsc_queue_1_history_agree with "Hhistory_auth Hhistory_at") as %Hlookup.
     iDestruct (xchain_model_lookup_acc with "Hhist") as "(Hnode & Hhist)"; first done.
     wp_load.
     iDestruct ("Hhist" with "Hnode ") as "Hhist".
     destruct (hist !! S i) as [node' |] eqn:Hlookup'; simpl.
 
     - iDestruct (big_sepL_lookup with "Hheaders") as "#Hnode'_hdr"; first done.
-      iDestruct (mpsc_queue_1_history_elem_get (S i) with "Hhistory_auth") as "#Hhistory_elem'"; first done.
+      iDestruct (mpsc_queue_1_history_at_get (S i) with "Hhistory_auth") as "#Hhistory_at'"; first done.
       destruct (decide (op = MpscQueue1IsEmpty)) as [-> | Hop].
 
       + iDestruct "Hop" as "(Hl_front_1 & HΨ & Hβ_empty & Hβ_nonempty)".
@@ -403,7 +403,7 @@ Section mpsc_queue_1_G.
     {{{
       meta l nroot γ ∗
       inv ι (mpsc_queue_1_inv_inner l γ) ∗
-      mpsc_queue_1_history_elem γ i node
+      mpsc_queue_1_history_at γ i node
     }}}
       (#node).{xchain_next}
     {{{ res,
@@ -412,11 +412,11 @@ Section mpsc_queue_1_G.
       ∨ ∃ node',
         ⌜res = #node'⌝ ∗
         node' ↦ₕ Header §Node 2 ∗
-        mpsc_queue_1_history_elem γ (S i) node'
+        mpsc_queue_1_history_at γ (S i) node'
     }}}.
   Proof.
-    iIntros "%Φ (#Hmeta & #Hinv & #Hhistory_elem) HΦ".
-    wp_apply (mpsc_queue_1_xchain_next_spec_strong MpscQueue1Other TeleO inhabitant inhabitant inhabitant inhabitant with "[$Hmeta $Hinv $Hhistory_elem //]").
+    iIntros "%Φ (#Hmeta & #Hinv & #Hhistory_at) HΦ".
+    wp_apply (mpsc_queue_1_xchain_next_spec_strong MpscQueue1Other TeleO inhabitant inhabitant inhabitant inhabitant with "[$Hmeta $Hinv $Hhistory_at //]").
     iSteps.
   Qed.
 
@@ -436,7 +436,7 @@ Section mpsc_queue_1_G.
   Proof.
     iIntros "!> %Φ ((%l & %γ & -> & #Hmeta & #Hinv) & (%_l & %front & %Heq & Hl_front)) HΦ". injection Heq as <-.
 
-    iMod (mpsc_queue_1_inv_inner_history_elem with "Hinv Hl_front") as "(%i & Hl_front & #Hfront_hdr & #Hhistory_elem)".
+    iMod (mpsc_queue_1_inv_inner_history_at with "Hinv Hl_front") as "(%i & Hl_front & #Hfront_hdr & #Hhistory_at)".
 
     iAssert (
       AU <{
@@ -457,7 +457,7 @@ Section mpsc_queue_1_G.
     }
 
     wp_rec. wp_load. wp_match.
-    wp_smart_apply (mpsc_queue_1_xchain_next_spec_strong MpscQueue1IsEmpty [tele_pair bool] _ [tele_arg true] [tele_arg false] with "[$Hmeta $Hinv $Hhistory_elem $Hl_front $HΦ]"); last iSteps.
+    wp_smart_apply (mpsc_queue_1_xchain_next_spec_strong MpscQueue1IsEmpty [tele_pair bool] _ [tele_arg true] [tele_arg false] with "[$Hmeta $Hinv $Hhistory_at $Hl_front $HΦ]"); last iSteps.
     iSplitR; iSteps.
   Qed.
 
@@ -466,7 +466,7 @@ Section mpsc_queue_1_G.
       meta l nroot γ ∗
       inv ι (mpsc_queue_1_inv_inner l γ) ∗
       node ↦ₕ Header §Node 2 ∗
-      mpsc_queue_1_history_elem γ i node ∗
+      mpsc_queue_1_history_at γ i node ∗
       new_back ↦ₕ Header §Node 2 ∗
       new_back.[xchain_next] ↦ () ∗
       new_back.[xchain_data] ↦ v
@@ -478,20 +478,20 @@ Section mpsc_queue_1_G.
       mpsc_queue_1_model #l (vs ++ [v])
     | RET ();
       ∃ j,
-      mpsc_queue_1_history_elem γ j new_back
+      mpsc_queue_1_history_at γ j new_back
     >>>.
   Proof.
-    iIntros "!> %Φ (#Hmeta & #Hinv & #Hnode_hdr & #Hhistory_elem & #Hnew_back_hdr & Hnew_back_next & Hnew_back_data) HΦ".
+    iIntros "!> %Φ (#Hmeta & #Hinv & #Hnode_hdr & #Hhistory_at & #Hnew_back_hdr & Hnew_back_next & Hnew_back_data) HΦ".
 
-    iLöb as "HLöb" forall (i node) "Hnode_hdr Hhistory_elem".
+    iLöb as "HLöb" forall (i node) "Hnode_hdr Hhistory_at".
 
     wp_rec. wp_match.
-    wp_smart_apply (mpsc_queue_1_xchain_next_spec with "[$Hmeta $Hinv $Hhistory_elem]") as (res) "[-> | (%node' & -> & #Hnode'_hdr & #Hhistory_elem')]". 2:{ wp_match. iSteps. }
+    wp_smart_apply (mpsc_queue_1_xchain_next_spec with "[$Hmeta $Hinv $Hhistory_at]") as (res) "[-> | (%node' & -> & #Hnode'_hdr & #Hhistory_at')]". 2:{ wp_match. iSteps. }
     wp_pures.
 
     wp_bind (CAS _ _ _).
     iInv "Hinv" as "(%hist & %past & %front & %nodes & %back & %vs & >%Hhist & >%Hback & Hl_front & Hl_back & Hhist & Hheaders & Hnodes & >Hhistory_auth & Hmodel₂)".
-    iDestruct (mpsc_queue_1_history_agree with "Hhistory_auth Hhistory_elem") as %Hlookup.
+    iDestruct (mpsc_queue_1_history_agree with "Hhistory_auth Hhistory_at") as %Hlookup.
     iDestruct (xchain_model_lookup with "Hhist") as "(Hhist1 & Hnode & Hhist2)"; first done.
     destruct (hist !! S i) as [node' |] eqn:Hlookup'; simpl.
 
@@ -507,7 +507,7 @@ Section mpsc_queue_1_G.
       iDestruct (big_sepL2_snoc with "[$Hnodes $Hnew_back_data]") as "Hnodes".
       iDestruct (xchain_model_snoc_2 with "Hhist Hnew_back_next") as "Hhist".
       iMod (mpsc_queue_1_history_update new_back with "Hhistory_auth") as "Hhistory_auth".
-      iDestruct (mpsc_queue_1_history_elem_get with "Hhistory_auth") as "#Hhistory_elem_new_back".
+      iDestruct (mpsc_queue_1_history_at_get with "Hhistory_auth") as "#Hhistory_at_new_back".
       { rewrite lookup_snoc_Some. naive_solver. }
       iMod "HΦ" as "(%_vs & (%_l & %_γ & %Heq & #_Hmeta & Hmodel₁) & _ & HΦ)". injection Heq as <-.
       iDestruct (meta_agree with "Hmeta _Hmeta") as %<-. iClear "_Hmeta".
@@ -527,9 +527,9 @@ Section mpsc_queue_1_G.
     {{{
       meta l nroot γ ∗
       inv ι (mpsc_queue_1_inv_inner l γ) ∗
-      mpsc_queue_1_history_elem γ i back ∗
+      mpsc_queue_1_history_at γ i back ∗
       new_back ↦ₕ Header §Node 2 ∗
-      mpsc_queue_1_history_elem γ j new_back
+      mpsc_queue_1_history_at γ j new_back
     }}}
       mpsc_queue_1_fix_back #l #back #new_back
     {{{
@@ -537,25 +537,25 @@ Section mpsc_queue_1_G.
       True
     }}}.
   Proof.
-    iIntros "%Φ (#Hmeta & #Hinv & #Hhistory_elem_back & #Hnew_back_hdr & #Hhistory_elem_new_back) HΦ".
+    iIntros "%Φ (#Hmeta & #Hinv & #Hhistory_at_back & #Hnew_back_hdr & #Hhistory_at_new_back) HΦ".
 
-    iLöb as "HLöb" forall (i back) "Hhistory_elem_back".
+    iLöb as "HLöb" forall (i back) "Hhistory_at_back".
 
     wp_rec. wp_match.
     wp_bind (_ and _)%E.
     wp_apply (wp_wand _ _ (λ res, ∃ b, ⌜res = #b⌝)%I) as (res) "(%b & ->)".
-    { wp_smart_apply (mpsc_queue_1_xchain_next_spec with "[$Hmeta $Hinv $Hhistory_elem_new_back]") as (res) "[-> | (%new_back' & -> & #Hnew_back'_hdr & #Hhistory_elem_new_back')]"; last iSteps.
+    { wp_smart_apply (mpsc_queue_1_xchain_next_spec with "[$Hmeta $Hinv $Hhistory_at_new_back]") as (res) "[-> | (%new_back' & -> & #Hnew_back'_hdr & #Hhistory_at_new_back')]"; last iSteps.
       wp_pures.
 
       wp_bind (CAS _ _ _).
       iInv "Hinv" as "(%hist & %past & %front & %nodes & %back' & %vs & >%Hhist & >%Hback & Hl_front & Hl_back & Hhist & Hheaders & Hnodes & Hhistory_auth & Hmodel₂)".
       wp_cas as _ | [= ->]; first iSteps.
-      iDestruct (mpsc_queue_1_history_agree with "Hhistory_auth Hhistory_elem_new_back") as %Hnew_back%elem_of_list_lookup_2.
+      iDestruct (mpsc_queue_1_history_agree with "Hhistory_auth Hhistory_at_new_back") as %Hnew_back%elem_of_list_lookup_2.
       iSteps.
     }
     destruct b; last iSteps.
-    wp_smart_apply (mpsc_queue_1_back_spec with "Hinv") as (back' i') "(_ & #Hhistory_elem_back')".
-    iApply ("HLöb" with "HΦ Hhistory_elem_back'").
+    wp_smart_apply (mpsc_queue_1_back_spec with "Hinv") as (back' i') "(_ & #Hhistory_at_back')".
+    iApply ("HLöb" with "HΦ Hhistory_at_back'").
   Qed.
 
   Lemma mpsc_queue_1_push_spec t ι v :
@@ -576,10 +576,10 @@ Section mpsc_queue_1_G.
     wp_rec.
     wp_block new_back as "#Hnew_back_hdr" "_" "(Hnew_back_next & Hnew_back_data & _)".
     wp_match.
-    wp_smart_apply (mpsc_queue_1_back_spec with "Hinv") as (back i) "(#Hback_hdr & #Hhistory_elem_back)".
-    wp_smart_apply (mpsc_queue_1_do_push_spec with "[$Hmeta $Hinv $Hhistory_elem_back $Hnew_back_hdr $Hnew_back_next $Hnew_back_data //]").
-    iApply (atomic_update_wand with "HΦ"). iIntros "%vs HΦ (%j & #Hhistory_elem_new_back)".
-    wp_smart_apply (mpsc_queue_1_fix_back_spec with "[$Hmeta $Hinv Hhistory_elem_back Hhistory_elem_new_back] HΦ").
+    wp_smart_apply (mpsc_queue_1_back_spec with "Hinv") as (back i) "(#Hback_hdr & #Hhistory_at_back)".
+    wp_smart_apply (mpsc_queue_1_do_push_spec with "[$Hmeta $Hinv $Hhistory_at_back $Hnew_back_hdr $Hnew_back_next $Hnew_back_data //]").
+    iApply (atomic_update_wand with "HΦ"). iIntros "%vs HΦ (%j & #Hhistory_at_new_back)".
+    wp_smart_apply (mpsc_queue_1_fix_back_spec with "[$Hmeta $Hinv Hhistory_at_back Hhistory_at_new_back] HΦ").
     iSteps.
   Qed.
 
@@ -601,10 +601,10 @@ Section mpsc_queue_1_G.
 
     iLöb as "HLöb".
 
-    iMod (mpsc_queue_1_inv_inner_history_elem with "Hinv Hl_front_1") as "(%i & Hl_front_1 & #Hfront_hdr & #Hhistory_elem)".
+    iMod (mpsc_queue_1_inv_inner_history_at with "Hinv Hl_front_1") as "(%i & Hl_front_1 & #Hfront_hdr & #Hhistory_at)".
 
     wp_rec. wp_load. wp_match.
-    wp_smart_apply (mpsc_queue_1_xchain_next_spec_strong MpscQueue1Pop _ _ [tele_arg] inhabitant with "[$Hmeta $Hinv $Hhistory_elem $Hl_front_1 $HΦ]") as (res) "[(-> & Hl_front_1 & HΦ) | (%new_front & -> & #Hnew_front_hdr & #Hhistory_elem_new & Hl_front_1 & HΦ)]"; [auto | iSteps |].
+    wp_smart_apply (mpsc_queue_1_xchain_next_spec_strong MpscQueue1Pop _ _ [tele_arg] inhabitant with "[$Hmeta $Hinv $Hhistory_at $Hl_front_1 $HΦ]") as (res) "[(-> & Hl_front_1 & HΦ) | (%new_front & -> & #Hnew_front_hdr & #Hhistory_at_new & Hl_front_1 & HΦ)]"; [auto | iSteps |].
     wp_match. wp_pures.
 
     wp_bind (Store _ _ _)%E.
@@ -615,8 +615,8 @@ Section mpsc_queue_1_G.
     wp_store.
     iEval (rewrite -Qp.three_quarter_quarter) in "Hl_front".
     iDestruct "Hl_front" as "(Hl_front_1 & Hl_front_2)".
-    iDestruct (mpsc_queue_1_history_agree with "Hhistory_auth Hhistory_elem") as %Hlookup.
-    iDestruct (mpsc_queue_1_history_agree with "Hhistory_auth Hhistory_elem_new") as %Hlookup_new.
+    iDestruct (mpsc_queue_1_history_agree with "Hhistory_auth Hhistory_at") as %Hlookup.
+    iDestruct (mpsc_queue_1_history_agree with "Hhistory_auth Hhistory_at_new") as %Hlookup_new.
     iAssert ⌜length past = i⌝%I as %Hpast_length.
     { iDestruct (xchain_model_NoDup with "Hhist") as %Hnodup.
       iPureIntro. eapply NoDup_lookup; try done.
